Translation/Uniqueness.v
@@ -4,162 +4,156 @@ From Coq Require Import Bool String List BinPos Compare_dec Omega.
 From Equations Require Import Equations DepElimDec.
 From Template Require Import Ast utils Typing.
 From Translation
-Require Import util SAst SLiftSubst Equality SCommon Conversion ITyping
-               ITypingInversions ITypingLemmata ContextConversion.
+Require Import util SAst SLiftSubst Equality SCommon ITyping ITypingLemmata.
 
 Ltac unitac h1 h2 :=
-  ttinv h1 ; ttinv h2 ;
-  eapply conv_trans ; [
-    eapply conv_sym ; eassumption
-  | idtac
-  ].
+  inversion h1 ; inversion h2 ; subst ; try eassumption ; try reflexivity.
 
 Lemma uniqueness :
   forall {Σ Γ A B u},
     type_glob Σ ->
     Σ ;;; Γ |-i u : A ->
     Σ ;;; Γ |-i u : B ->
-    Σ |-i A = B.
+    A = B.
 Proof.
   intros Σ Γ A B u hg h1 h2.
   revert Γ A B h1 h2.
   induction u ; intros Γ A B h1 h2.
   all: try unitac h1 h2. all: try assumption.
-  - cbn in *. erewrite @safe_nth_irr with (isdecl' := is) in h0. assumption.
-  - specialize (IHu1 _ _ _ h h0).
-    specialize (IHu2 _ _ _ h4 h7).
-    eapply conv_trans ; try eapply h6.
-    pose proof (sort_conv_inv IHu1) as e1.
-    pose proof (sort_conv_inv IHu2) as e2.
-    subst. apply conv_refl.
-  - eapply nl_conv ; try eassumption ; reflexivity.
-  - specialize (IHu1 _ _ _ h0 h6).
-    pose proof (sort_conv_inv IHu1) as e. subst. assumption.
-  - specialize (IHu1 _ _ _ h h0).
-    pose proof (sort_conv_inv IHu1) as e. subst. assumption.
-  - specialize (IHu _ _ _ h h0).
-    pose proof (heq_conv_inv IHu) as e. split_hyps.
-    eapply conv_trans ; try exact h8.
-    apply cong_Eq ; assumption.
-  - specialize (IHu _ _ _ h4 h10).
-    pose proof (heq_conv_inv IHu) as e. split_hyps.
-    eapply conv_trans ; [ | exact h9 ].
-    apply cong_Heq ; assumption.
-  - specialize (IHu1 _ _ _ h5 h14).
-    specialize (IHu2 _ _ _ h4 h13).
-    pose proof (heq_conv_inv IHu1) as e1.
-    pose proof (heq_conv_inv IHu2) as e2. split_hyps.
-    eapply conv_trans ; [ | exact h12 ].
-    apply cong_Heq ; assumption.
-  - specialize (IHu1 _ _ _ h4 h9).
-    specialize (IHu2 _ _ _ h5 h10).
-    pose proof (eq_conv_inv IHu1) as e1. split_hyps.
-    eapply conv_trans ; [| exact h8 ].
-    apply cong_Heq ; try assumption.
-    + apply conv_refl.
-    + apply cong_Transport ; try assumption.
-      all: apply conv_refl.
-  - specialize (IHu3 _ _ _ h h0).
-    pose proof (heq_conv_inv IHu3) as e3. split_hyps.
-    pose proof (sort_conv_inv pi1_). subst.
-    assert (hh : Σ ;;; Γ,, A1 |-i u1 : sSort z0).
-    { eapply type_ctxconv ; try eassumption.
-      - econstructor ; try eassumption.
-        eapply typing_wf. eassumption.
-      - constructor.
-        + apply ctxconv_refl.
-        + apply conv_sym. assumption.
-    }
-    specialize (IHu1 _ _ _ h5 hh).
-    pose proof (sort_conv_inv IHu1). subst.
-    eapply conv_trans ; [| exact h10 ].
-    apply cong_Heq.
-    + apply conv_refl.
-    + apply cong_Prod ; try assumption.
-      apply conv_refl.
-    + apply conv_refl.
-    + apply cong_Prod ; try assumption. apply conv_refl.
-  - specialize (IHu5 _ _ _ h0 h12).
-    pose proof (heq_conv_inv IHu5) as e5. split_hyps.
-    pose proof (sort_conv_inv pi1_). subst.
-    eapply conv_trans ; [| exact h13 ].
-    apply cong_Heq ; try assumption.
-    + apply cong_Prod ; try assumption. apply conv_refl.
-    + apply cong_Lambda ; try assumption. all: apply conv_refl.
-    + apply cong_Prod ; try assumption. apply conv_refl.
-    + apply cong_Lambda ; try assumption. all: apply conv_refl.
-  - specialize (IHu3 _ _ _ h13 h26).
-    specialize (IHu4 _ _ _ h h0).
-    specialize (IHu6 _ _ _ h12 h25).
-    pose proof (heq_conv_inv IHu3).
-    pose proof (heq_conv_inv IHu4).
-    pose proof (heq_conv_inv IHu6).
-    split_hyps.
-    eapply conv_trans ; [| exact h16 ].
-    apply cong_Heq ; try assumption.
-    + apply substs_conv. assumption.
-    + apply cong_App ; try assumption. apply conv_refl.
-    + apply substs_conv. assumption.
-    + apply cong_App ; try assumption. apply conv_refl.
-  - specialize (IHu1 _ _ _ h0 h12).
-    specialize (IHu2 _ _ _ h11 h21).
-    specialize (IHu3 _ _ _ h10 h20).
-    pose proof (heq_conv_inv IHu1).
-    pose proof (heq_conv_inv IHu2).
-    pose proof (heq_conv_inv IHu3).
-    split_hyps. subst.
-    eapply conv_trans ; [| exact h13 ].
-    apply cong_Heq ; try assumption.
-    + apply cong_Eq ; assumption.
-    + apply cong_Eq ; assumption.
-  - specialize (IHu1 _ _ _ h h0).
-    specialize (IHu2 _ _ _ h8 h15).
-    pose proof (heq_conv_inv IHu1).
-    pose proof (heq_conv_inv IHu2).
-    split_hyps.
-    pose proof (sort_conv_inv pi1_0). subst.
-    eapply conv_trans ; [| exact h10 ].
-    apply cong_Heq.
-    + apply cong_Eq ; assumption.
-    + apply cong_Refl ; assumption.
-    + apply cong_Eq ; assumption.
-    + apply cong_Refl ; assumption.
-  - specialize (IHu _ _ _ h h0).
-    pose proof (eq_conv_inv IHu). split_hyps.
-    eapply conv_trans ; [| exact h8 ].
-    apply cong_Heq ; assumption.
-  - specialize (IHu1 _ _ _ h7 h13).
-    specialize (IHu3 _ _ _ h0 h8).
-    apply conv_sym in IHu1. pose proof (sort_conv_inv IHu1). subst.
-    pose proof (heq_conv_inv IHu3). split_hyps.
-    eapply conv_trans ; [| exact h9 ].
-    apply cong_Eq ; assumption.
-  - specialize (IHu1 _ _ _ h h0).
-    eapply conv_trans ; [| exact h6 ].
-    assumption.
-  - specialize (IHu _ _ _ h4 h8).
-    pose proof (pack_conv_inv IHu).
-    split_hyps.
-    eapply conv_trans ; [| exact h7 ].
-    assumption.
-  - specialize (IHu _ _ _ h4 h8).
-    pose proof (pack_conv_inv IHu).
-    split_hyps.
-    eapply conv_trans ; [| exact h7 ].
-    assumption.
-  - specialize (IHu _ _ _ h4 h8).
-    pose proof (pack_conv_inv IHu).
-    split_hyps.
-    eapply conv_trans ; [| exact h7 ].
-    apply cong_Heq ; try assumption ; apply conv_refl.
-  - eapply conv_trans ; [| exact h0 ].
-    destruct isdecl as [d1 [[hd1 ?] hn1]].
-    destruct isdecl0 as [d2 [[hd2 ?] hn2]].
-    unfold sdeclared_minductive in *.
-    rewrite hd1 in hd2. inversion hd2. subst.
-    rewrite hn1 in hn2. inversion hn2. subst.
-    apply conv_refl.
-  - eapply conv_trans ; [| exact h0 ].
-    erewrite SCommon.stype_of_constructor_eq. apply conv_refl.
-  - ttinv h1.
-Defined.
+  - cbn in *. erewrite @safe_nth_irr with (isdecl' := isdecl0) in *. reflexivity.
+  - specialize (IHu1 _ _ _ H4 H11).
+    specialize (IHu2 _ _ _ H5 H12).
+    inversion IHu1. inversion IHu2.
+    subst. reflexivity.
+  (* - eapply nl_conv ; try eassumption ; reflexivity. *)
+  (* - specialize (IHu1 _ _ _ h0 h6). *)
+  (*   pose proof (sort_conv_inv IHu1) as e. subst. assumption. *)
+  (* - specialize (IHu1 _ _ _ h h0). *)
+  (*   pose proof (sort_conv_inv IHu1) as e. subst. assumption. *)
+  (* - specialize (IHu _ _ _ h h0). *)
+  (*   pose proof (heq_conv_inv IHu) as e. split_hyps. *)
+  (*   eapply conv_trans ; try exact h8. *)
+  (*   apply cong_Eq ; assumption. *)
+  (* - specialize (IHu _ _ _ h4 h10). *)
+  (*   pose proof (heq_conv_inv IHu) as e. split_hyps. *)
+  (*   eapply conv_trans ; [ | exact h9 ]. *)
+  (*   apply cong_Heq ; assumption. *)
+  (* - specialize (IHu1 _ _ _ h5 h14). *)
+  (*   specialize (IHu2 _ _ _ h4 h13). *)
+  (*   pose proof (heq_conv_inv IHu1) as e1. *)
+  (*   pose proof (heq_conv_inv IHu2) as e2. split_hyps. *)
+  (*   eapply conv_trans ; [ | exact h12 ]. *)
+  (*   apply cong_Heq ; assumption. *)
+  (* - specialize (IHu1 _ _ _ h4 h9). *)
+  (*   specialize (IHu2 _ _ _ h5 h10). *)
+  (*   pose proof (eq_conv_inv IHu1) as e1. split_hyps. *)
+  (*   eapply conv_trans ; [| exact h8 ]. *)
+  (*   apply cong_Heq ; try assumption. *)
+  (*   + apply conv_refl. *)
+  (*   + apply cong_Transport ; try assumption. *)
+  (*     all: apply conv_refl. *)
+  (* - specialize (IHu3 _ _ _ h h0). *)
+  (*   pose proof (heq_conv_inv IHu3) as e3. split_hyps. *)
+  (*   pose proof (sort_conv_inv pi1_). subst. *)
+  (*   assert (hh : Σ ;;; Γ,, A1 |-i u1 : sSort z0). *)
+  (*   { eapply type_ctxconv ; try eassumption. *)
+  (*     - econstructor ; try eassumption. *)
+  (*       eapply typing_wf. eassumption. *)
+  (*     - constructor. *)
+  (*       + apply ctxconv_refl. *)
+  (*       + apply conv_sym. assumption. *)
+  (*   } *)
+  (*   specialize (IHu1 _ _ _ h5 hh). *)
+  (*   pose proof (sort_conv_inv IHu1). subst. *)
+  (*   eapply conv_trans ; [| exact h10 ]. *)
+  (*   apply cong_Heq. *)
+  (*   + apply conv_refl. *)
+  (*   + apply cong_Prod ; try assumption. *)
+  (*     apply conv_refl. *)
+  (*   + apply conv_refl. *)
+  (*   + apply cong_Prod ; try assumption. apply conv_refl. *)
+  (* - specialize (IHu5 _ _ _ h0 h12). *)
+  (*   pose proof (heq_conv_inv IHu5) as e5. split_hyps. *)
+  (*   pose proof (sort_conv_inv pi1_). subst. *)
+  (*   eapply conv_trans ; [| exact h13 ]. *)
+  (*   apply cong_Heq ; try assumption. *)
+  (*   + apply cong_Prod ; try assumption. apply conv_refl. *)
+  (*   + apply cong_Lambda ; try assumption. all: apply conv_refl. *)
+  (*   + apply cong_Prod ; try assumption. apply conv_refl. *)
+  (*   + apply cong_Lambda ; try assumption. all: apply conv_refl. *)
+  (* - specialize (IHu3 _ _ _ h13 h26). *)
+  (*   specialize (IHu4 _ _ _ h h0). *)
+  (*   specialize (IHu6 _ _ _ h12 h25). *)
+  (*   pose proof (heq_conv_inv IHu3). *)
+  (*   pose proof (heq_conv_inv IHu4). *)
+  (*   pose proof (heq_conv_inv IHu6). *)
+  (*   split_hyps. *)
+  (*   eapply conv_trans ; [| exact h16 ]. *)
+  (*   apply cong_Heq ; try assumption. *)
+  (*   + apply substs_conv. assumption. *)
+  (*   + apply cong_App ; try assumption. apply conv_refl. *)
+  (*   + apply substs_conv. assumption. *)
+  (*   + apply cong_App ; try assumption. apply conv_refl. *)
+  (* - specialize (IHu1 _ _ _ h0 h12). *)
+  (*   specialize (IHu2 _ _ _ h11 h21). *)
+  (*   specialize (IHu3 _ _ _ h10 h20). *)
+  (*   pose proof (heq_conv_inv IHu1). *)
+  (*   pose proof (heq_conv_inv IHu2). *)
+  (*   pose proof (heq_conv_inv IHu3). *)
+  (*   split_hyps. subst. *)
+  (*   eapply conv_trans ; [| exact h13 ]. *)
+  (*   apply cong_Heq ; try assumption. *)
+  (*   + apply cong_Eq ; assumption. *)
+  (*   + apply cong_Eq ; assumption. *)
+  (* - specialize (IHu1 _ _ _ h h0). *)
+  (*   specialize (IHu2 _ _ _ h8 h15). *)
+  (*   pose proof (heq_conv_inv IHu1). *)
+  (*   pose proof (heq_conv_inv IHu2). *)
+  (*   split_hyps. *)
+  (*   pose proof (sort_conv_inv pi1_0). subst. *)
+  (*   eapply conv_trans ; [| exact h10 ]. *)
+  (*   apply cong_Heq. *)
+  (*   + apply cong_Eq ; assumption. *)
+  (*   + apply cong_Refl ; assumption. *)
+  (*   + apply cong_Eq ; assumption. *)
+  (*   + apply cong_Refl ; assumption. *)
+  (* - specialize (IHu _ _ _ h h0). *)
+  (*   pose proof (eq_conv_inv IHu). split_hyps. *)
+  (*   eapply conv_trans ; [| exact h8 ]. *)
+  (*   apply cong_Heq ; assumption. *)
+  (* - specialize (IHu1 _ _ _ h7 h13). *)
+  (*   specialize (IHu3 _ _ _ h0 h8). *)
+  (*   apply conv_sym in IHu1. pose proof (sort_conv_inv IHu1). subst. *)
+  (*   pose proof (heq_conv_inv IHu3). split_hyps. *)
+  (*   eapply conv_trans ; [| exact h9 ]. *)
+  (*   apply cong_Eq ; assumption. *)
+  (* - specialize (IHu1 _ _ _ h h0). *)
+  (*   eapply conv_trans ; [| exact h6 ]. *)
+  (*   assumption. *)
+  (* - specialize (IHu _ _ _ h4 h8). *)
+  (*   pose proof (pack_conv_inv IHu). *)
+  (*   split_hyps. *)
+  (*   eapply conv_trans ; [| exact h7 ]. *)
+  (*   assumption. *)
+  (* - specialize (IHu _ _ _ h4 h8). *)
+  (*   pose proof (pack_conv_inv IHu). *)
+  (*   split_hyps. *)
+  (*   eapply conv_trans ; [| exact h7 ]. *)
+  (*   assumption. *)
+  (* - specialize (IHu _ _ _ h4 h8). *)
+  (*   pose proof (pack_conv_inv IHu). *)
+  (*   split_hyps. *)
+  (*   eapply conv_trans ; [| exact h7 ]. *)
+  (*   apply cong_Heq ; try assumption ; apply conv_refl. *)
+  (* - eapply conv_trans ; [| exact h0 ]. *)
+  (*   destruct isdecl as [d1 [[hd1 ?] hn1]]. *)
+  (*   destruct isdecl0 as [d2 [[hd2 ?] hn2]]. *)
+  (*   unfold sdeclared_minductive in *. *)
+  (*   rewrite hd1 in hd2. inversion hd2. subst. *)
+  (*   rewrite hn1 in hn2. inversion hn2. subst. *)
+  (*   apply conv_refl. *)
+  (* - eapply conv_trans ; [| exact h0 ]. *)
+  (*   erewrite SCommon.stype_of_constructor_eq. apply conv_refl. *)
+  (* - ttinv h1. *)
+(* Defined. *)
+Admitted.
